src/ForWord.v
@@ -1,0 +1,12 @@
+Require Import bbv.Word.
+
+Notation "'for' m 'from' 0 'to' N 'updating' ( s1 ) {{ b }} ;; rest" :=
+  (let s1 :=
+    (fix rec(n: nat) := match n with
+     | 0 => s1
+     | S m => let s1 := rec m in
+              let m := natToWord _ m in
+              b
+     end) (wordToNat N)
+  in rest)
+  (at level 20, right associativity).
